fstar/Interpreter.fst
@@ -18,12 +18,61 @@ let rec interpret_exp env exp = match exp with
 	  | Times -> op_Multiply vleft vright
 
 
-type low_equiv (label_env:label_env) (e1:value_env) (e2:value_env) =
-  forall x. lookup_env label_env x == Low ==> (lookup_env e1 x) == (lookup_env e2 x)
+type low_equiv (lenv:label_env) (e1:value_env) (e2:value_env) =
+  forall (x:var). is_low lenv x ==> lookup_env e1 x == lookup_env e2 x
+
+type ni_exp (lenv:label_env) (exp:exp) =
+  forall (e1:value_env) (e2:value_env). low_equiv lenv e1 e2 ==> interpret_exp e1 exp == interpret_exp e2 exp
+
+
+val low_equiv_symmetric : lenv:label_env -> e1:value_env -> e2:value_env ->
+  Lemma (requires (low_equiv lenv e1 e2))
+        (ensures  (low_equiv lenv e2 e1))
+let low_equiv_symmetric _ _ _ = ()
+
+
+val ni_int : lenv:label_env -> n:int ->
+  Lemma (requires True)
+        (ensures (ni_exp lenv (Int n)))
+let ni_int _ _ = ()
+
+
+val ni_low_var : lenv:label_env -> var:var ->
+  Lemma (requires (is_low lenv var))
+        (ensures (ni_exp lenv (Var var)))
+let ni_low_var _ _ = ()
+
+
+val var_lemma : var:var -> n:int ->
+  Lemma (requires True)
+        (ensures (interpret_exp (make_env 0 [(var, n)]) (Var var) = n))
+let var_lemma _ _ = ()
+
+
+val low_equiv_hi : lenv:label_env -> e1:value_env -> e2:value_env -> var:var ->
+  Lemma (requires ((low_equiv lenv e1 e2) /\ (lookup_env e1 var) =!= (lookup_env e2 var)))
+        (ensures (is_high lenv var))
+let low_equiv_hi _ _ _ _ = ()
+
+
+val ni_high_var : lenv:label_env -> var:var ->
+  Lemma (requires (is_high lenv var))
+        (ensures (~ (ni_exp lenv (Var var))))
+let ni_high_var lenv var =
+  let exp = Var var in
+  let e1 = make_env 0 [(var, 0)] in
+  let e2 = make_env 0 [(var, 1)] in
+	low_equiv_hi lenv e1 e2 var
+
+
+val ni_binop : lenv:label_env -> op:binop -> exp1:exp -> exp2:exp ->
+  Lemma (requires (ni_exp lenv exp1 /\ ni_exp lenv exp2))
+        (ensures (ni_exp lenv (BinOp exp1 op exp2)))
+let ni_binop _ _ _ _ = ()
 
 
 let _ =
-	let lenv = make_env Low [("lo", Low); ("hi", High)] in
+	let lenv = make_env Low [("lo", Low); ("lo2", Low); ("hi", High)] in
 
 	let lo_env = (update_env empty_value_env "lo" 10) in
 	let hi_env = (update_env empty_value_env "hi" 7) in
@@ -34,4 +83,16 @@ let _ =
 	assert (empty_equiv empty_value_env);
 	assert (~ (empty_equiv lo_env));
 	assert (empty_equiv hi_env);
-	assert (empty_equiv lo2_env)
+	assert (empty_equiv lo2_env);
+
+	let exp_int = Int 10 in
+
+	assert (ni_exp lenv exp_int);
+
+	let exp  = (BinOp (Var "lo") Plus (BinOp (Var "lo2") Times (Int 7))) in
+	let exp' = (BinOp (Var "hi") Minus (Var "hi")) in
+	let exp'' = (BinOp (Var "hi") Times (Int 0)) in
+
+	assert (ni_exp lenv exp);
+	assert (ni_exp lenv exp');
+	assert (ni_exp lenv exp'')
